big idgaf update

Jrlean/Coc/VarOffseting.lean
@@ -3,6 +3,9 @@ module
 public import Jrlean.Coc.Var
 public import Jrlean.Coc.VarConversions
 public import Jrlean.Coc.Offseting
+public import Jrlean.Coc.Shadows
+public import Jrlean.Coc.VarInc
+public import Jrlean.Coc.VarDec
 
 import Jrlean.Of
 
@@ -13,48 +16,14 @@ public section
 
 variable {varKind : VarKind}
 
-abbrev DVar := @Var .deBruijn
-abbrev NVar := @Var .named
-
--- Offset In
-
-@[grind]
-def Var.offsetInDeBruijn (v bound : DVar) : DVar :=
-  if v.toNat < bound.toNat then v
-  else v.toNat + 1
-
-@[grind]
-def Var.offsetInNamed (v bound : NVar) : NVar :=
-  if v.name != bound.name then v
-  else if v.depth < bound.depth then v
-  else ⟨v.name, v.depth + 1⟩
-
 @[grind]
 def Var.offsetIn (v bound : @Var varKind) : Var' :=
-  match varKind with
-  | .deBruijn => v.offsetInDeBruijn bound
-  | .named => v.offsetInNamed bound
-
--- Offset Out
-
-@[grind]
-def Var.offsetOutDeBruijn (v : DVar) (unbound : DVar) : Option DVar :=
-  if v = unbound then none
-  else if v.toNat > unbound then some of v.toNat - 1
-  else some v
-
-@[grind]
-def Var.offsetOutNamed (v : NVar) (unbound : NVar) : Option NVar :=
-  if v.name != unbound.name then v
-  else if v.depth = unbound.depth then none
-  else if v.depth > unbound.depth then some ⟨v.name, v.depth - 1⟩
-  else v
+  if bound ≤ v then v++ else v
 
 @[grind]
 def Var.offsetOut (v unbound : @Var varKind) : Option Var' :=
-  match varKind with
-  | .deBruijn => v.offsetOutDeBruijn unbound
-  | .named => v.offsetOutNamed unbound
+  if unbound = v then none
+  else some of if unbound < v then v- else v
 
 instance : Offset varKind Var' where
   offsetIn v bound := v.offsetIn bound
