Jrlean/Coc/VarOffsetInLemmas.lean
@@ -1,0 +1,66 @@
+module
+
+public import Jrlean.Coc.VarOffseting
+public import Jrlean.Coc.Shadowed
+
+import Jrlean.Coc.ShadowedLemmas
+import Jrlean.Coc.ShadowsLemmas
+import Jrlean.Coc.VarIncLemmas
+import Jrlean.Coc.VarDecLemmas
+
+namespace Jrlean.Coc.Var
+
+public section
+
+variable {varKind : VarKind}
+variable {x y z : Var'}
+
+@[grind =]
+theorem offsetIn_eq : x↑y = if y ≤ x then x++ else x := rfl
+@[grind =, simp]
+theorem offsetIn_of_shadowsEq (h : y ≤ x) : x↑y = x++ := by grind only [= offsetIn_eq]
+@[grind =]
+theorem offsetIn_eq_inc_iff : x↑y = x++ ↔ y ≤ x := by
+  grind only [= offsetIn_of_shadowsEq, = offsetIn_eq, inc_neq, #d0c7]
+@[grind =, simp]
+theorem offsetIn_of_not_shadowsEq (h : ¬(y ≤ x)) : x↑y = x := by grind only [= offsetIn_eq]
+theorem offsetIn_eq_iff : x↑y = x ↔ ¬(y ≤ x) := by
+    grind only [= offsetIn_of_not_shadowsEq, = offsetIn_of_shadowsEq, = offsetIn_eq_inc_iff, inc_neq]
+grind_pattern offsetIn_eq_iff => x↑y where x =?= x↑y
+
+@[grind ., simp]
+theorem shadowsEq_offsetIn : x ≤ x↑y := by
+  grind only [= offsetIn_of_not_shadowsEq, = offsetIn_of_shadowsEq, → neq_of_shadows,
+    = offsetIn_eq_inc_iff, → shadowsEq_right_trans, shadows_inc, #82de]
+
+@[grind =, simp]
+theorem shadows_offsetIn_iff : x < x↑y ↔ y ≤ x := by
+  grind only [→ neq_of_shadows, shadowsEq_offsetIn, = offsetIn_of_shadowsEq, = offsetIn_eq,
+    = offsetIn_eq_inc_iff, inc_neq, #6985]
+
+@[grind =_, simp]
+theorem offsetIn_neq_iff : x↑y ≠ x ↔ x↑y = x++ := by
+  grind only [= offsetIn_of_not_shadowsEq, = offsetIn_eq_inc_iff, inc_neq, #3797]
+@[grind =, simp]
+theorem offsetIn_neq_inc_iff : x↑y ≠ x++ ↔ x↑y = x := by
+  grind only [=_ offsetIn_neq_iff]
+
+@[grind =, simp]
+theorem inc_offsetIn : (x↑y)++ = (x++)↑(y++) := by
+  grind =>
+    instantiate only [= inc_inj, = offsetIn_neq_inc_iff, =_ offsetIn_neq_iff, = offsetIn_eq_inc_iff,
+      = offsetIn_eq]
+    instantiate only [= offsetIn_neq_inc_iff, = offsetIn_eq_inc_iff, shadowsEq_inc_iff_shadows]
+    instantiate only [= shadows_inc_iff_shadowsEq]
+    cases #c50d
+@[grind =, simp]
+theorem dec_offsetIn (h_x : x.Shadowed) (h_y : y.Shadowed) : (x↑y)- = (x-)↑(y-) := by
+  grind =>
+    instantiate only [= dec_inj, = offsetIn_of_shadowsEq, = offsetIn_eq]
+    instantiate only [= shadows_dec_iff_shadowsEq, = offsetIn_eq_inc_iff, =_ offsetIn_neq_iff,
+      = offsetIn_neq_inc_iff, = inc_dec]
+    instantiate only [=> shadowsEq_dec_iff_shadows]
+    cases #aa1a
+    · instantiate only [= shadowed_iff_zero_lt]
+      cases #8c23 <;> instantiate only [= dec_inc]
+    · cases #8c23 <;> instantiate only [= dec_inc]
