Jrlean/Coc/VarOffsetOutLemmas.lean
@@ -1,0 +1,20 @@
+module
+
+public import Jrlean.Coc.VarOffseting
+
+import Jrlean.Coc.ShadowedLemmas
+import Jrlean.Coc.ShadowsLemmas
+import Jrlean.Coc.VarIncLemmas
+import Jrlean.Coc.VarDecLemmas
+import Jrlean.Coc.VarOffsetInLemmas
+
+namespace Jrlean.Coc.Var
+
+public section
+
+variable {varKind : VarKind}
+variable {x y z : Var'}
+
+-- TODO
+
+theorem offsetOut_eq : x↓y = if y = x then none else x := rfl
