Jrlean/Coc/VarOffsetingLemmas.lean
@@ -2,7 +2,13 @@ module
 
 public import Jrlean.Coc.VarOffseting
 
+import Jrlean.Coc.ShadowsLemmas
+import Jrlean.Coc.ShadowedLemmas
+import Jrlean.Coc.VarIncLemmas
+import Jrlean.Coc.VarDecLemmas
+
 import Jrlean.SetTactic
+import Jrlean.ByContra
 
 namespace Jrlean.Coc
 
@@ -15,10 +21,6 @@ variable {v v' v'' x y z : Var'}
 attribute [local grind .]
   Var.offsetIn
   Var.offsetOut
-  Var.offsetInDeBruijn
-  Var.offsetInNamed
-  Var.offsetOutDeBruijn
-  Var.offsetOutNamed
   Offset.offsetIn
   Offset.offsetOut
   NamedVar.ext
@@ -30,19 +32,18 @@ attribute [local grind .]
 theorem Var.offsetOut_isSome_of_neq
     (h : v ≠ v')
     : (v↓v').isSome := by
-  grind only [= eq_2, = offsetOut_notation, offsetOut, offsetOutDeBruijn, = Option.isSome_some, offsetOutNamed,
-    NamedVar.ext, #aa1a, #616e, #75b3, #9840]
+  grind only [= offsetOut_notation, offsetOut, = Option.isSome_some]
 grind_pattern Var.offsetOut_isSome_of_neq => v↓v'
 
 @[grind =, simp]
 theorem Var.offsetOut_eq_none : v↓v = none := by
-  grind only [= offsetOut_notation, offsetOut, offsetOutDeBruijn, offsetOutNamed, #aa1a]
+  grind only [= offsetOut_notation, offsetOut]
 
 @[grind =, simp]
 theorem Var.offsetOut_isSome
     : (v↓v').isSome = (v ≠ v') := by
-  grind only [usr offsetOut_isSome_of_neq, = offsetOut_notation, offsetOut, offsetOutDeBruijn,
-    = Option.isSome_none, offsetOutNamed, #5af2, #aa1a]
+  grind only [usr offsetOut_isSome_of_neq, = offsetOut_notation, offsetOut, = Option.isSome_none,
+    #5af2]
 
 @[simp]
 theorem Var.offsetOut_eq_some_of_neq
@@ -55,47 +56,53 @@ grind_pattern Var.offsetOut_eq_some_of_neq => v↓v'
 /-- Offseting in never gives the same variable as the rhs. -/
 @[grind ., simp]
 theorem Var.offsetIn_neq : v↑v' ≠ v' := by
-  grind only [= offsetIn_notation, offsetIn, offsetInDeBruijn, offsetInNamed, #aa1a, #0019, #46c1,
-    #8585]
+  if h : v = v' then
+    grind only [= offsetIn_notation, offsetIn, → neq_of_shadows, shadows_inc]
+  else
+    simp only [Offset.offsetIn, offsetIn]
+    grind only [shadowsEq_inc_iff_shadows, → neq_of_shadows, #d94a]
 
 @[grind =, simp]
 theorem Var.offsetOut_offsetIn : (v↑v')↓v' = some v := by
-  set vIn := v↑v' with h_vIn
-  have : vIn ≠ v' := by subst vIn; exact offsetIn_neq
-  show vIn.offsetOut v' = some v
-  cases varKind
-  case deBruijn =>
-    rw [offsetOut, offsetOutDeBruijn]
-    rw [toNat]
-    rw [ite_cond_eq_false (h := eq_false this)]
-    rw [←apply_ite]
-    rw [Option.some_inj]
-    if h : toNat v < v' then
-      have : vIn = v := by grind only [= offsetIn_notation, offsetIn, offsetInDeBruijn]
-      clear h_vIn
-      subst vIn
-      have : ¬ toNat v > v' := by grind only
-      rw [if_neg this]
-    else
-      have h_vIn : vIn = toNat v + 1 := by grind only [= offsetIn_notation, offsetIn,
-        offsetInDeBruijn]
-      have : toNat vIn > v' := by grind only
-      rw [if_pos this]
-      rw [h_vIn]
-      rfl
-  case named =>
-    sorry
+  grind =>
+    instantiate only [usr offsetOut_eq_some_of_neq, = offsetOut_notation, offsetIn_neq,
+      = offsetIn_notation]
+    instantiate only [offsetOut, offsetIn]
+    cases #aa1a
+    · instantiate only [= shadows_iff_lt]
+      cases #3bc3 <;>
+        cases #d94a <;>
+          instantiate only [= shadows_inc_iff_shadowsEq] <;> instantiate only [= dec_inc]
+    · instantiate only [= shadows_iff_name_eq_and_depth_lt]
+      instantiate only [→ not_shadows_of_name_neq]
+      instantiate only [→ shadowsEq_right_trans, → shadowsEq_trans]
+      cases #3bc3 <;>
+        cases #d94a <;> instantiate only [shadows_inc] <;> instantiate only [= dec_inc]
 
 @[grind =, simp]
 theorem Var.offsetIn_offsetOut_of_isSome
     (h : (v↓v').isSome)
-    : (v↓v').bind (·↓v') = some v := by
-  sorry
+    : (v↓v').map (·↑v') = some v := by
+  if h₁ : v < v' then
+    grind only [= offsetOut_isSome, = offsetOut_notation, offsetOut, → shadows_trans,
+      = Option.map_some, → neq_of_shadows, = offsetIn_notation, offsetIn]
+  else if h₂ : v' < v then
+    grind only [= offsetOut_isSome, usr offsetOut_eq_some_of_neq, = offsetOut_notation,
+      → shadowed_of_shadows, → neq_of_shadows, offsetOut, =_ not_unshadowed_iff_shadowed,
+      = not_shadowed_iff_unshadowed, = Option.map_some, = offsetIn_notation, offsetIn,
+      = shadows_iff_lt, = shadowed_iff_zero_lt, => shadowsEq_dec_iff_shadows,
+      = unshadowed_iff_eq_zero, = inc_dec, = shadows_iff_name_eq_and_depth_lt, shadowsEq_antisymm,
+      = dec_eq_with_pred_depth, = shadows_dec_iff_shadowsEq, NamedVar.ext, #aa1a, #a87d, #f0d2,
+      #2864]
+  else
+    grind only [= offsetOut_isSome, = offsetOut_notation, offsetOut, = Option.map_some,
+      = offsetIn_notation, offsetIn]
 
 @[grind =]
 theorem Var.offsetIn_offsetOut_eq_ite
-    : (v↓v').bind (·↓v') = if v = v' then none else some v := by
-  sorry
+    : (v↓v').map (·↑v') = if v = v' then none else some v := by
+  grind only [= offsetIn_offsetOut_of_isSome, = offsetOut_notation, = offsetOut_isSome, offsetOut,
+    = Option.map_none, #3ced]
 
 @[grind =]
 theorem Var.bind_offsetOut_eq_ite
@@ -110,8 +117,10 @@ theorem Var.bind_offsetOut_eq_ite
 @[grind =]
 theorem Var.offsetOut_offsetOut_of_isSome
     (h : (x↓y).isSome)
-    : (x↓y).get!↓z = (x↓(z↑y)).bind (·↓y) :=
-  sorry
+    (h : (y↓z).isSome)
+    : (x↓y).get!↓z = (x↓(z↑y)).bind (·↓(y↓z).get!) := by
+  simp_all
+  grind
 
 @[grind =, simp]
 theorem Var.offsetOut_eq_none_iff : v↓v' = none ↔ v = v' := by
@@ -125,12 +134,12 @@ theorem Var.offsetOut_eq_none_iff : v↓v' = none ↔ v = v' := by
 theorem Var.offsetOut_bind_offsetOut : (x↓y).bind (·↓z) = (x↓(z↑y)).bind (·↓(y↑z)) := by
   rw [Var.bind_offsetOut_eq_ite]
   split
-  · sorry
-  -- · subst y
-  --   symm
-  --   rw [Option.bind_eq_none_iff]
-  --   intro x' h
-  --   rw [offsetOut_eq_none_iff]
+  · subst y
+    symm
+    rw [Option.bind_eq_none_iff]
+    intro x' h
+    rw [offsetOut_eq_none_iff]
+    simp_all
   · sorry
 
 /-- A very obvious theorem, that makes grind case-split when needed. -/
